preuves

examples/Sek/PArray_proof.v
@@ -146,10 +146,67 @@ Notation "'LetFun' f ':=' B1 'in' F1" :=
 Ltac xcf_pre tt ::=
 	intros; match goal with |- TripleMon _ _ _ _ => unfold TripleMon | _ => idtac end.
 
+#[global]
+Hint Rewrite @LibMap.dom_update : rew_map.
+
+Hint Extern 1 (dom _ \c dom _) => rew_map; set_prove.
+Hint Extern 1 (_ \in dom _) => rew_map; set_prove.
+Hint Extern 1 (?x <> ?y :> loc) => 
+	match goal with 
+	| H1: ?x \in ?E, H2: ~ ?y \in ?E |- _ => intros ->; false 
+	| H1: ~ ?x \in ?E, H2: ?y \in ?E |- _ => intros ->; false 
+	end.
+
+Lemma xsimpl_l_false : forall Nc Hla Hlw Hlt HR,
+  Xsimpl (Nc, Hla, Hlw, (\[False] \* Hlt)) HR.
+Proof using.
+	intros. apply xsimpl_l_hpure. intros. false.
+Qed.
+
+Ltac xsimpl_step_l tt ::=
+	match goal with |- Xsimpl ?HL ?HR =>
+	match HL with
+	| (?Nc, ?Hla, ?Hlw, (?H \* ?Hlt)) =>
+		match H with
+		| \[] => apply xsimpl_l_hempty
+		| \[False] => apply xsimpl_l_false
+		| \[?P] => apply xsimpl_l_hpure; intro
+		| \$ ?n => apply xsimpl_l_hcredits
+		| ?H1 \* ?H2 => rewrite (@hstar_assoc H1 H2)
+		| hexists ?J => apply xsimpl_l_hexists; intro
+		| ?H1 \-* ?H2 => apply xsimpl_l_acc_hwand
+		| ?Q1 \--* ?Q2 => apply xsimpl_l_acc_hwand
+		| _ => apply xsimpl_l_acc_other
+		end
+	| (?Nc, ?Hla, ((?H1 \-* ?H2) \* ?Hlw), \[]) =>
+			match H1 with
+			| \[] => apply xsimpl_l_cancel_hwand_hempty
+			| \$ ?n => apply xsimpl_l_hwand_hcredits
+			| (_ \* _) => xsimpl_hwand_hstars_l tt
+			| _ => first [ xsimpl_pick_same H1; apply xsimpl_l_cancel_hwand
+									 | apply xsimpl_l_keep_wand ]
+			end
+	| (?Nc, ?Hla, ((?Q1 \--* ?Q2) \* ?Hlw), \[]) =>
+			first [ xsimpl_pick_applied Q1; eapply xsimpl_l_cancel_qwand
+						| apply xsimpl_l_keep_wand ]
+	end end.
+
+Ltac set_prove2 := (* set_prove fails sometimes *)
+	set_prove_setup false; intuition.
+
+
+Parameter copy_spec : forall A `{EA:Enc A} (xs:list A) t,
+  SPEC (Array_ml.copy t)
+    INV (t ~> Array xs)
+    POST (fun t' => t' ~> Array xs).
+
+Hint Extern 1 (RegisterSpec Array_ml.copy) => Provide copy_spec.
+
 
 
 (*************************************************)
 (** PArrays *)
+
 Implicit Types p q: loc.
 
 (* parray_desc *)
@@ -180,24 +237,23 @@ Lemma PArray_Desc_eq : forall A (EA: Enc A) (D: Desc A) (d: parray_desc_ A),
 Proof using. auto. Qed.
 
 Lemma PArray_Desc_eq_Base : forall A (EA: Enc A) (D: Desc A) (a: array A),
-	PArray_Base a ~> PArray_Desc D = \exists L, \[D = Desc_Base L] \* a ~> Array L.
+	(PArray_Base a) ~> PArray_Desc D = \exists L, \[D = Desc_Base L] \* a ~> Array L.
 Proof using.
-	intros. cases D; rewrite PArray_Desc_eq.
-	{ xsimpl*. intros L E. injection E. auto. }
-	{ xsimpl*. Unshelve. apply nil. (* Pourquoi il a besoin qu'on fasse ça ? *) }
+	intros. destruct D; rewrite PArray_Desc_eq.
+	{ xsimpl*. intros L E. inverts* E. }
+	{ xsimpl*. }
 Qed.
 
 Lemma PArray_Desc_eq_Diff : forall A (EA: Enc A) (D: Desc A) p i x,
-	PArray_Diff p i x ~> PArray_Desc D = \[D = Desc_Diff p i x].
+	(PArray_Diff p i x) ~> PArray_Desc D = \[D = Desc_Diff p i x].
 Proof using.
-	intros. cases D; rewrite PArray_Desc_eq.
+	intros. destruct D; rewrite PArray_Desc_eq.
 	{	xsimpl*. }
-	{ xsimpl*; intros H; injection H as E1 E2 E3; subst; auto. }
+	{ xsimpl*; intros H; inverts* H. }
 Qed.
 
+
 Hint Extern 1 (RegisterOpen PArray_Desc) => Provide PArray_Desc_eq.
-
-
 
 
 Definition PArray A {EA: Enc A} (D: Desc A) (pa: parray_ A) : hprop :=
@@ -208,14 +264,18 @@ Lemma PArray_eq : forall A (pa: parray_ A) (EA: Enc A) (D: Desc A),
 	\exists d, pa ~~~> `{ data' := d } \* d ~> PArray_Desc D.
 Proof using. auto. Qed.
 
+Lemma PArray_Base_close : forall A (EA: Enc A) (pa: parray_ A) (a: array A) (L: list A),
+	pa ~~~> `{ data' := PArray_Base a } \* a ~> Array L ==> pa ~> PArray (Desc_Base L).
+Proof using. intros. xchange* <- PArray_Desc_eq_Base. xchange* <- PArray_eq. Qed.
+
+
 Hint Extern 1 (RegisterOpen PArray) => Provide PArray_eq.
 
 Global Instance Heapdata_PArray : forall A (EA: Enc A),
 	Heapdata (PArray (A := A)).
 Proof using.
 	intros. apply Heapdata_intro. intros.
-	xchange* PArray_eq. intros D2.
-	xchange* PArray_eq. intros D1.
+	do 2 xchange* PArray_eq.
 	xchange* Heapdata_record.
 Qed.
 
@@ -224,34 +284,119 @@ Hint Resolve Heapdata_PArray.
 
 Notation "'Memory' A" := (map (parray_ A) (Desc A)) (at level 69).
 
+Inductive IsPArray A {IA: Inhab A} {EA: Enc A} (M: Memory A) : list A -> parray_ A -> Prop :=
+	|	IsPArray_Base : forall pa L,
+			pa \indom M ->
+			M[pa] = Desc_Base L ->
+			IsPArray M L pa
+	|	IsPArray_Diff : forall pa' pa i x L' L,
+			pa \indom M ->
+			M[pa] = Desc_Diff pa' i x ->
+			IsPArray M L' pa' ->
+			index L' i ->
+			L = L'[i := x] ->
+			IsPArray M L pa.
+
+Lemma IsPArray_inv_indom : forall A (IA: Inhab A) (EA: Enc A) (M: Memory A) (pa: parray_ A) (L: list A),
+	IsPArray M L pa ->
+	pa \indom M.
+Proof using. intros. inverts* H. Qed.
+
+Hint Resolve IsPArray_inv_indom.
+
+Section IsPArray_sized.
+
+Inductive IsPArray_sized A {IA: Inhab A} {EA: Enc A} (M: Memory A) : list A -> parray_ A -> nat -> Prop :=
+	|	IsPArray_Base_sized : forall pa L,
+			pa \indom M ->
+			M[pa] = Desc_Base L ->
+			IsPArray_sized M L pa 0
+	|	IsPArray_Diff_sized : forall pa' pa i x L' L n,
+			pa \indom M ->
+			M[pa] = Desc_Diff pa' i x ->
+			IsPArray_sized M L' pa' n ->
+			index L' i ->
+			L = L'[i := x] ->
+			IsPArray_sized M L pa (S n).
+
+Hint Constructors IsPArray IsPArray_sized.
+
+Lemma IsPArray_sized_of_unsized : forall A (IA: Inhab A) (EA: Enc A) (M: Memory A) (L: list A) (pa: parray_ A),
+	IsPArray M L pa -> exists n, IsPArray_sized M L pa n.
+Proof using. introv H. induction* H. Qed.
+
+Lemma IsPArray_unsized_of_sized : forall A (IA: Inhab A) (EA: Enc A) (M: Memory A) (L: list A) (pa: parray_ A) (n: nat),
+	IsPArray_sized M L pa n -> IsPArray M L pa.
+Proof using. introv H. induction* H. Qed.
+
+End IsPArray_sized.
+
+Hint Resolve IsPArray_unsized_of_sized.
+
+
 Record Inv A {IA: Inhab A} {EA: Enc A} (M: Memory A) : Prop := {
-	Inv_closure : forall p,
+	Inv_closure : forall p i v q,
 		p \indom M ->
-		forall i v q, M[p] = Desc_Diff q i v ->
+		M[p] = Desc_Diff q i v ->
 		q \indom M
 }.
 
-Inductive IsPArray A {IA: Inhab A} {EA: Enc A} (M: Memory A) : list A -> parray_ A -> Prop :=
-|	IsPArray_Base : forall pa L,
-		pa \indom M ->
-		M[pa] = Desc_Base L ->
-		IsPArray M L pa
-|	IsPArray_Diff : forall pa pa' i x L L',
-		pa \indom M ->
-		M[pa] = Desc_Diff pa' i x ->
-		IsPArray M L' pa' ->
-		L = L'[i := x] ->
-		IsPArray M L pa.
+Definition Points_into {A} {IA: Inhab A} {EA: Enc A} (M: Memory A) (D: Desc A) : Prop :=
+	match D with
+	|	Desc_Base _ => True
+	|	Desc_Diff q _ _ => q \indom M
+	end.
 
-Lemma IsPArray_inv_indom : forall A (IA: Inhab A) (EA: Enc A) (M: Memory A) (pa: parray_ A) (L: list A),
-	IsPArray M L pa -> pa \indom M.
-Proof using. intros. inversion H; auto. Qed.
+Lemma Points_into_Base : forall A (IA: Inhab A) (EA: Enc A) (M: Memory A) (L: list A),
+	Points_into M (Desc_Base L).
+Proof using. unfold Points_into. auto. Qed.
 
-Hint Resolve IsPArray_inv_indom.
+Lemma Points_into_eq_Diff : forall A (IA: Inhab A) (EA: Enc A) (M: Memory A) q i x,
+	Points_into M (Desc_Diff q i x) = q \indom M.
+Proof using. unfold Points_into. auto. Qed.
+
+Hint Resolve Points_into_Base Points_into_eq_Diff.
 
 
 Definition Shared {A} {IA: Inhab A} {EA: Enc A} (M: Memory A) : hprop :=
 	Group (PArray (A := A)) M \* \[Inv M].
+
+Lemma Shared_inv_Inv : forall A (IA: Inhab A) (EA: Enc A) (M: Memory A),
+	Shared M ==+> \[Inv M].
+Proof using. unfold Shared. xsimpl*. Qed.
+
+Lemma Shared_inv_focus : forall A (IA: Inhab A) (EA: Enc A) (M: Memory A) (pa: parray_ A) (L: list A),
+	IsPArray M L pa ->
+	Shared M ==>
+		\[Inv M] \*
+		pa ~> PArray (M[pa]) \*
+		\forall D,
+			pa ~> PArray D \-*
+			\[Points_into M D] \-*
+			Shared (M[pa := D]).
+Proof using.
+	intros. unfold Shared. xchange* (>> Group_focus pa).
+	intros Inv. xsimpl*; intros D.
+	{ destruct D; intros C; constructors*; intros p i v q Hdom E.
+		{ rewrites* read_update in E. case_if*.
+			rew_map in *. forwards*: Inv_closure p; [set_prove2 | set_prove]. }
+		{ rewrites* read_update in E. case_if*.
+			{ inverts* E. }
+			{ rew_map in *. forwards*: Inv_closure p; [set_prove2 | set_prove]. } } }
+	{ xchange* (>> hforall_specialize D). }
+Qed.
+
+Lemma Shared_add_fresh_Base : forall A (IA: Inhab A) (EA: Enc A) (M: Memory A) (pa: parray_ A) (L: list A),
+	pa ~> PArray (Desc_Base L) \* Shared M ==> Shared (M[pa := Desc_Base L]) \* \[pa \notindom M].
+Proof using.
+	skip.
+Qed.
+
+Lemma Shared_add_fresh_Diff : forall A (IA: Inhab A) (EA: Enc A) (M: Memory A) (pa: parray_ A) q i x,
+	pa ~> PArray (Desc_Diff q i x) \* \[q \indom M] \* Shared M ==> Shared (M[pa := Desc_Diff q i x]) \* \[pa \notindom M].
+Proof using.
+	skip.
+Qed.
 
 
 Definition Extend {A} {IA: Inhab A} {EA: Enc A} (M M': Memory A) : Prop :=
@@ -259,48 +404,29 @@ Definition Extend {A} {IA: Inhab A} {EA: Enc A} (M M': Memory A) : Prop :=
 
 Lemma IsPArray_extend : forall A (IA: Inhab A) (EA: Enc A) (M M': Memory A) p L,
 	Extend M M' -> IsPArray M L p -> IsPArray M' L p.
-Proof. introv [_ H] Arr. auto. Qed.
+Proof using. introv [_ H] Arr. auto. Qed.
 
+Lemma Extend_id : forall A (IA: Inhab A) (EA: Enc A) (M: Memory A),
+	Extend M M.
+Proof using. unfold Extend. auto. Qed.
 
-Instance MonType_EChunkMap A {IA: Inhab A} {EA: Enc A} :
+Lemma Extend_add_fresh : forall A (IA: Inhab A) (EA: Enc A) (M: Memory A) (pa: parray_ A) (D: Desc A),
+	~(pa \indom M) ->
+		Extend M (M[pa := D]).
+Proof using.
+	introv H. unfold Extend. split*.
+	{ intros L p Rp. induction Rp.
+		{ applys* IsPArray_Base. rew_map*. }
+		{ applys* IsPArray_Diff. rew_map*. } }
+Qed.
+
+Instance MonType_Memory A {IA: Inhab A} {EA: Enc A} :
 	MonType (Memory A) :=	make_MonType (Shared) (Extend).
 
 (*************************************************)
 (** Specifications *)
 
-Lemma focus_shared : forall A (IA: Inhab A) (EA: Enc A) (M: Memory A) (pa: parray_ A) (L: list A),
-  IsPArray M L pa ->
-  Shared M ==+> pa ~> PArray M[pa].
-Proof using.
-  skip.
-Qed.
-
-#[global]
-Hint Rewrite @LibMap.dom_update : rew_map.
-
-Hint Extern 1 (dom _ \c dom _) => rew_map; set_prove.
-Hint Extern 1 (_ \in dom _) => rew_map; set_prove.
-Hint Extern 1 (?x <> ?y :> loc) => 
-  match goal with 
-  | H1: ?x \in ?E, H2: ~ ?y \in ?E |- _ => intros ->; false 
-  | H1: ~ ?x \in ?E, H2: ?y \in ?E |- _ => intros ->; false 
-  end.
-
-
-
-Lemma Extend_add_binding : forall A (IA: Inhab A) (EA: Enc A) (M: Memory A) (pa: parray_ A) (D: Desc A),
-	~(pa \indom M) ->
-		Extend M (M[pa := D]).
-Proof using.
-	introv H. unfold Extend. split.
-	{ auto. (* rew_map. set_prove. *) }
-	{ intros L p Rp. induction Rp.
-		{ apply IsPArray_Base.
-			{ auto. (* rew_map. set_prove. *) }
-			{ rew_map*. (* intros ->. false*. *) } }
-		{ applys* IsPArray_Diff. rew_map*. } }
-Qed.
-
+(* Laisser tel quel *)
 Lemma parray_create_spec : forall A (IA: Inhab A) (EA: Enc A) (M: Memory A) (sz: int) (d: A),
 	sz >= 0 ->
 	SPEC (parray_create sz d)
@@ -310,26 +436,12 @@ Lemma parray_create_spec : forall A (IA: Inhab A) (EA: Enc A) (M: Memory A) (sz:
 Proof using.
 	introv Hsz. xcf*. simpl.
 	xpay_skip.
-	xapp*. intros a L E. subst.
+	xapp*. intros a L ->.
 	xapp*. intros pa.
-
-	xchange* <- PArray_Desc_eq_Base. 
-	xchange* <- PArray_eq.
-	unfold Shared.
-	xchange* (>> Group_add_fresh pa).
-	{ apply Heapdata_PArray. }
-	{
-		(* Lemme Shared M ==+> Inv M. *)
-		intros Inv. lets [Inv_closure]: Inv.
-		intros Hnot_indom. xsimpl*.
-		{ apply* Extend_add_binding. }
-		{ constructors*.
-			{ intros p Hindom i x q H.
-				rewrites* read_update in H. case_if* in H.
-				forwards* Clos: Inv_closure H.
-				{ forwards* [|]: indom_update_inv Hindom; tryfalse. }
-				(*{ rewrites* (>> indom_update_eq M). }*) } }
-		{ applys* IsPArray_Base. rew_map*. } }
+	xchange* PArray_Base_close.
+	xchanges* Shared_add_fresh_Base; intros Hpa.
+	{ apply* Extend_add_fresh. }
+	{ apply* IsPArray_Base. rew_map*. }
 Qed.
 
 Hint Extern 1 (RegisterSpec parray_create) => Provide parray_create_spec.
@@ -347,19 +459,29 @@ Lemma parray_base_copy_spec : forall A (IA: Inhab A) (EA: Enc A) (M: Memory A) (
 		INV (Shared M)
 		POST (fun a => a ~> Array L).
 Proof using.
-	introv Harr. induction Harr; xcf*; xpay_skip.
-	{ xchange* (>> focus_shared M pa L).
-		{ apply* IsPArray_Base. }
-		{ xopen* pa. intros d. xapp*. xcase; cases M[pa].
-			{ cases* M[pa]; auto. (* Spec de copy ? *) skip. }
-			{ skip. } } }
-	{ xchange* (>> focus_shared M pa L).
-		{ apply* IsPArray_Diff. }
-		{ xopen* pa. intros d. xapp*. xcase.
-			{ (* Contradiction ? *) skip. }
-			{ xcase.
-				{ skip. }
-				{ xdone. } } } }
+	introv Rpa. lets (n&Rpas): IsPArray_sized_of_unsized Rpa.
+	gen pa L. induction_wf IH: wf_lt n.
+	introv Rpa. xcf*. xpay_skip.
+	xchange* Shared_inv_focus. intros Inv.
+	xopen* pa. intros D. xapp*. xmatch.
+	{ xchange* PArray_Desc_eq_Base. intros L' E.
+		inverts* Rpas; tryfalse.
+		rewrite E in H0. inverts* H0.
+		xapp*. intros q. xsimpl*.
+		xchange* PArray_Base_close.
+		xchange* hforall_specialize.
+		xchange* hwand_hpure_l.
+		rewrites* <- E. rew_map*. xsimpl*. }
+	{ xchange* PArray_Desc_eq_Diff. intros E.
+		inverts Rpas; tryfalse.
+		rewrite E in H0. inverts* H0.
+		xchange* <- PArray_Desc_eq_Diff. xclose* pa.
+		xchange* hforall_specialize.
+		rewrites* E. rewrites* Points_into_eq_Diff.
+		xchange* hwand_hpure_l.
+		{ applys* Inv_closure Inv. }
+		{ rewrites* <- E. rew_map*.
+			xapp* IH; try math. intros a. xapp*. xval*. xsimpl*. } }
 Qed.
 
 Hint Extern 1 (RegisterSpec parray_base_copy) => Provide parray_base_copy_spec.
@@ -367,9 +489,29 @@ Hint Extern 1 (RegisterSpec parray_base_copy) => Provide parray_base_copy_spec.
 Lemma parray_rebase_and_get_array_spec : forall A (IA: Inhab A) (EA: Enc A) (M: Memory A) (pa: parray_ A) (L: list A),
 	IsPArray M L pa ->
 	SPEC (parray_rebase_and_get_array pa)
-		INV (Shared M)
-		POST (fun a => a ~> Array L \* \[M[pa] = Desc_Base L]).
-Admitted.
+		MONO M
+		PRE \[]
+		POST (fun M' a =>
+			a ~> Array L \*
+			\[IsPArray M' L pa] \*
+			\[M'[pa] = Desc_Base L]).
+Proof using.
+	introv Rpa. xcf*. xpay_skip.
+	xchange* Shared_inv_focus. intros Inv.
+	xopen* pa. intros D. xapp*. xmatch.
+	{ xval*.
+		xchange* PArray_Desc_eq_Base.
+		intros L' E.
+		inverts* Rpa; tryfalse.
+		rewrite E in H0. inverts* H0.
+		xsimpl*.
+		(* xchange* PArray_Base_close. *)
+		xchange* (hforall_specialize (M[pa])).
+		rewrites* E.
+		xchange* hwand_hpure_l.
+		rewrites* <- E. rew_map*.
+		xsimpl*. }
+Qed.
 
 Hint Extern 1 (RegisterSpec parray_rebase_and_get_array) => Provide parray_rebase_and_get_array_spec.
 
@@ -396,17 +538,7 @@ Lemma parray_set_spec : forall A (IA: Inhab A) (EA: Enc A) (M: Memory A) (pa: pa
 		POST (fun M' q => \[IsPArray M' (L[i := x]) q]).
 Proof using.
 	introv Harr Hind. xcf*. simpl. xpay_skip.
-	xchange* focus_shared. xopen* pa. intros D.
-	xapp*. intros a H. subst.
-	xapp*. intros q.
-	xappn*. xval.
-	xsimpl* M[q := Desc_Base L[i := x]].
-	{ apply Extend_add_binding; skip. }
-	{ apply IsPArray_Base.
-		{ apply* indom_update_same. }
-		{ rewrite* read_update_same. } }
-	{ xsimpl. }
-	(* Déplier le code de set ? *) skip.
+	skip.
 Qed.
 
 Hint Extern 1 (RegisterSpec parray_set) => Provide parray_set_spec.
